Crypto.v
@@ -1,0 +1,402 @@
+(** 
+Perfect Crypto - Simple definitions for message encryption and signing using
+symmetric and assymetric keys
+
+Perry Alexander
+The University of Kansas
+
+Provides definitions for:
+
+- [keyType] - [symmetric], [public] and [private] key constructors.
+- [inverse] - defines the inverse of any key.
+- [is_inverse] - proof that [inverse] is decidable and provides a decision procesure for [inverse].
+- [is_not_decryptable] - predicate indicating that a message is or is not decryptable using a specified key.
+- [decrypt] - attempts to decrypt a message with a given key.  Returns the decrypted message if decryption occurs.  Returns a proof that the message cannot be decrypted with the key if decryption does not occur.
+- [is_signed] - proof that signature checking is decidable and provides a decision procedure for signature check.
+- [check] - checks a signature on a message with a given key.  Returns a proof that the check succeeds or does not succeed.
+- [check_dec] - proof that signature checking is decidable and provides a decision procedure for signature checking.  Alternative function for [check].
+*)
+
+Require Import Omega.
+Require Import Ensembles.
+
+(** Ltac helper functions for discharging cases generated from sumbool types
+  using one or two boolean cases. *)
+
+Ltac eq_not_eq P := destruct P;
+  [ (left; subst; reflexivity) |
+    (right; unfold not; intros; inversion H; contradiction) ].
+
+Ltac eq_not_eq' P Q := destruct P; destruct Q;
+  [ (subst; left; reflexivity) |
+    (right; unfold not; intros; inversion H; contradiction) |
+    (right; unfold not; intros; inversion H; contradiction) |
+    (right; unfold not; intros; inversion H; contradiction) ].
+
+(** Key values will be [nat] by default.  Could be anything satisfying
+ properties following.  *)
+
+Definition key_val : Type := nat.
+
+(** Key types are [symmetric], [public] and [private]. *)
+Inductive keyType: Type :=
+| symmetric : key_val -> keyType
+| private : key_val -> keyType
+| public : key_val -> keyType.
+
+(** A [symmetric] key is its own inverse.  A [public] key is the inverse of
+  the [private] key with the same [key_val].  A [private] key is the inverse of
+  the [public] key with the same [key_val]. *)
+
+Fixpoint inverse(k:keyType):keyType :=
+match k with
+| symmetric k => symmetric k
+| public k => private k
+| private k => public k
+end.
+
+(** Proof that inverse is decidable for any two keys. The resulting proof
+ gives us the function [is_inverse] that is a decision procedure for key 
+ inverse checking.  It will be used in [decrypt] and [check] later in the
+ specification. *)
+
+Ltac is_inverse_helper :=
+  match goal with
+  | [ |- {symmetric ?P = (inverse (symmetric ?Q))}+{symmetric ?P <> (inverse (symmetric ?Q))} ] => (eq_not_eq (eq_nat_dec P Q))
+  | [ |- {private ?P = (inverse (public ?Q))}+{private ?P <> (inverse (public ?Q))} ] => (eq_not_eq (eq_nat_dec P Q))
+  | [ |- {public ?P = (inverse (private ?Q))}+{public ?P <> (inverse (private ?Q))} ] => (eq_not_eq (eq_nat_dec P Q))
+  | [ |- _ ] => right; simpl; unfold not; intros; inversion H
+  end.
+
+Theorem is_inverse:forall k k', {k = (inverse k')}+{k <> (inverse k')}.
+Proof.
+  intros.
+  destruct k; destruct k'; is_inverse_helper.
+Defined.
+
+Eval compute in (is_inverse (public 1) (private 1)).
+
+Eval compute in (is_inverse (public 1) (private 2)).
+
+Eval compute in (is_inverse (public 2) (private 1)).
+
+Eval compute in (is_inverse (private 1) (public 1)).
+
+Eval compute in (is_inverse (symmetric 1) (symmetric 1)).
+
+Eval compute in (is_inverse (symmetric 1) (symmetric 2)).
+
+(** Various proofs for keys and properties of the inverse operation.  All keys
+  must have an inverse.  All keys have a unique inverse.  Equal inverses come
+  from equal keys *)
+
+Theorem inverse_injective : forall k1 k2, inverse k1 = inverse k2 -> k1 = k2.
+Proof.
+  intros.
+  destruct k1; destruct k2; simpl in H; try (inversion H); try (reflexivity).
+Qed.
+
+Hint Resolve inverse_injective.
+
+Theorem inverse_inverse : forall k, inverse (inverse k) = k.
+Proof.
+  intros. destruct k; try reflexivity.
+Qed.
+
+Hint Resolve inverse_inverse.
+
+Theorem inverse_surjective : forall k, exists k', (inverse k) = k'.
+Proof.
+  intros. exists (inverse k). auto.
+Qed.
+
+Hint Resolve inverse_surjective.
+
+Theorem inverse_bijective : forall k k',
+    inverse k = inverse k' ->
+    k = k' /\ forall k, exists k'', inverse k = k''.
+Proof.
+  auto.
+Qed.
+
+(** Basic messages are natural numbers.  Really should be held abstract, but we
+  need an equality decision procedure to determine message equality.  Compound 
+  messages are keys, encrypted messages, hashes and pairs. Note that signed
+  messages are pairs of a message and encrypted hash. *) 
+
+Inductive message : Type :=
+| basic : nat -> message
+| key : keyType -> message
+| encrypt : message -> keyType -> message
+| hash : message -> message
+| pair : message -> message -> message.
+
+(** Predicate that determines if a message cannot be decrypted.  Could be
+  that it is not encrypted to begin with or the wrong key is used. *)
+
+Definition is_not_decryptable(m:message)(k:keyType):Prop :=
+  match m with
+  | encrypt m' k' => k <> inverse k'
+  | _ => True
+  end.
+
+Definition is_decryptable(m:message)(k:keyType):Prop :=
+  match m with
+  | encrypt m' k' => k = inverse k'
+  | _ => False
+  end.
+
+(** Prove that is_not_decryptable and is_decryptable are inverses.  This is a
+  bit sloppy.  Should really only have one or the other, but this theorem
+  assures they play together correctly.  Note that it is not installed as
+  a Hint.  *)
+
+Theorem decryptable_inverse: forall m k,
+    (is_not_decryptable m k) <-> (is_decryptable m k) -> False.
+Proof.
+  intros. split.
+  intros; destruct m; try (simpl in H; simpl in H0; contradiction).
+  intros. destruct m; try reflexivity.
+    simpl. simpl in H. unfold not. assumption.
+Qed.
+
+(** [decrypt] returns either a decrypted message or a proof of why the message
+  cannot be decrypted.  Really should be able to shorten the proof. *)
+
+Fixpoint decrypt(m:message)(k:keyType):message+{(is_not_decryptable m k)}.
+refine
+  match m with
+  | basic _ => inright _ _
+  | key _ => inright _ _
+  | encrypt m' j => (if (is_inverse k j) then (inleft _ m') else (inright _ _ ))
+  | hash _ => inright _ _
+  | pair _ _ => inright _ _
+  end.
+Proof.
+  reflexivity.
+  reflexivity.
+  simpl. assumption.
+  reflexivity.
+  reflexivity.
+Defined.
+
+(** This should solve the previous proof if there is a way to try it on every
+  proof generated by refine
+
+  repeat try (match goal with
+  | [ |- is_not_decryptable (encrypt ?X ?Y) ?Z ] => simpl; assumption
+  | [ |- _ ] => reflexivity
+  end).
+*)
+
+Eval compute in decrypt(encrypt (basic 1) (symmetric 1)) (symmetric 1).
+
+Eval compute in decrypt(encrypt (basic 1) (symmetric 1)) (symmetric 2).
+
+(** Generate a signature using encryption and hash *)
+
+Definition sign(m:message)(k:keyType):message :=
+  (pair m (encrypt (hash m) k)).
+
+Ltac eq_key_helper :=
+  match goal with
+  | [ |- {symmetric ?P = symmetric ?Q} + {symmetric ?P <> symmetric ?Q} ] =>
+    (eq_not_eq (eq_nat_dec P Q))
+  | [ |- {public ?P = public ?Q} + {public ?P <> public ?Q} ] =>
+    (eq_not_eq (eq_nat_dec P Q))
+  | [ |- {private ?P = private ?Q} + {private ?P <> private ?Q} ] =>
+    (eq_not_eq (eq_nat_dec P Q))
+  | [ |- _ ] => right; unfold not; intros; inversion H
+  end.
+
+Theorem eq_key_dec: forall k k':keyType, {k=k'}+{k<>k'}.
+Proof.
+  intros.
+  destruct k; destruct k'; eq_key_helper.
+Defined.
+  
+Hint Resolve eq_key_dec.
+
+Theorem message_eq_lemma: forall m m' k k',
+    {m=m'}+{m<>m'} ->
+    {k=k'}+{k<>k'} ->
+    {(encrypt m k)=(encrypt m' k')}+{(encrypt m k) <> (encrypt m' k')}.
+Proof.
+  intros.
+  destruct H; destruct H0;
+  match goal with
+  | [ |- {encrypt ?m ?k = encrypt ?m' ?k'} + {encrypt ?m ?k <> encrypt ?m' ?k'} ] => left; subst; reflexivity
+  | [ |- _ ] => right; unfold not; intros; inversion H; contradiction
+  end.
+Qed.
+
+Hint Resolve message_eq_lemma.
+
+Theorem message_eq_dec_orig: forall m m':message, {m=m'}+{m<>m'}.
+Proof.
+  induction m,m'.
+  destruct (eq_nat_dec n n0).
+    left. subst. reflexivity.
+    right. unfold not. intros. inversion H. contradiction.
+  right. unfold not. intros. inversion H.
+  right. unfold not. intros. inversion H.
+  right. unfold not. intros. inversion H.
+  right. unfold not. intros. inversion H.
+  right. unfold not. intros. inversion H.
+  destruct (eq_key_dec k k0).
+    left. subst. reflexivity.
+    right. unfold not. intros. inversion H. contradiction.
+  right. unfold not. intros. inversion H.
+  right. unfold not. intros. inversion H.
+  right. unfold not. intros. inversion H.
+  right. unfold not. intros. inversion H.
+  right. unfold not. intros. inversion H.
+  specialize IHm with m'.
+  apply message_eq_lemma. assumption. apply eq_key_dec.
+  right. unfold not. intros. inversion H.
+  right. unfold not. intros. inversion H.
+  right. unfold not. intros. inversion H.
+  right. unfold not. intros. inversion H.
+  right. unfold not. intros. inversion H.
+  specialize IHm with m'.
+  destruct IHm.
+  left. subst. reflexivity.
+  right. unfold not. intros. inversion H. contradiction.
+  right. unfold not. intros. inversion H.
+  right. unfold not. intros. inversion H.
+  right. unfold not. intros. inversion H.
+  right. unfold not. intros. inversion H.
+  right. unfold not. intros. inversion H.
+  specialize IHm1 with m'1.
+  specialize IHm2 with m'2.
+  destruct IHm1; destruct IHm2.
+  subst. left. reflexivity.
+  right. unfold not. intros. inversion H. contradiction.
+  right. unfold not. intros. inversion H. contradiction.
+  right. unfold not. intros. inversion H. contradiction.
+Defined.
+
+Ltac whack_right :=
+  match goal with
+  | [ |- {basic ?P = basic ?Q}+{basic ?P <> basic ?Q} ] =>
+    (eq_not_eq (eq_nat_dec P Q))
+  | [ |- {key ?P = key ?Q}+{key ?P <> key ?Q} ] =>
+    (eq_not_eq (eq_key_dec P Q))
+  | [ |- {encrypt ?P ?P' = encrypt ?Q ?Q'}+{encrypt ?P ?P' <> encrypt ?Q ?Q'} ] =>
+    auto 
+  | [ H : {?P = ?Q}+{?P <> ?Q} |- {hash ?P = hash ?Q}+{hash ?P <> hash ?Q} ] =>
+    (eq_not_eq H)
+  | [ H1 : {?P = ?P'}+{?P <> ?P'},
+      H2 : {?Q = ?Q'}+{?Q <> ?Q'}
+      |- {pair ?P ?Q = pair ?P' ?Q'}+{pair ?P ?Q <> pair ?P' ?Q'} ] =>
+    (eq_not_eq' H1 H2)
+  | [ |- _ ] => right; unfold not; intros; inversion H
+  end.
+
+Theorem message_eq_dec: forall m m':message, {m=m'}+{m<>m'}.
+Proof.
+  induction m; induction m';
+  try (specialize (IHm m'));
+  try (specialize (IHm1 m'1));
+  try (specialize (IHm2 m'2));
+  whack_right.
+Defined.
+
+Hint Resolve message_eq_dec.
+
+Theorem is_hash_dec: forall m h, {h=(hash m)}+{h<>(hash m)}.
+Proof.
+  intros.
+  destruct (message_eq_dec h (hash m)).
+  left. assumption.
+  right. assumption.
+Defined.
+
+Hint Resolve is_hash_dec.
+
+Definition is_signed(m:message)(k:keyType):Prop :=
+  match m with
+  | (pair m m') => match m' with
+                  | encrypt m'' k' =>  match m'' with
+                                      | (hash m''') => m=m''' /\ (k = inverse k')
+                                      | _ => False
+                                      end
+                  | _ => False
+                  end
+  | _ => False
+  end.
+
+Example sign_1_ex: is_signed (pair (basic 1) (encrypt (hash (basic 1)) (private 1))) (public 1).
+Proof.
+  simpl. tauto.
+Qed.
+
+Example sign_2_ex: not (is_signed (pair (basic 1) (encrypt (hash (basic 1)) (private 1))) (public 2)).
+Proof.
+  unfold not. intros.
+  simpl in H. inversion H. inversion H1.
+Qed.
+
+Theorem check_dec: forall m:message, forall k, {(is_signed m k)}+{not (is_signed m k)}.
+Proof.
+  intros.
+  destruct m.
+  tauto.
+  tauto.
+  tauto.
+  tauto.
+  destruct m2.
+    tauto.
+    tauto.
+    destruct m2.
+      tauto.
+      tauto.
+      tauto.
+      destruct (is_inverse k k0).
+        destruct (message_eq_dec m1 m2).
+        left. subst. simpl. tauto.
+          right. unfold not. intros. simpl in H. tauto.
+          right. unfold not. intros. simpl in H. tauto.
+      tauto.
+      tauto.
+      tauto.
+Defined.
+            
+Eval compute in check_dec (sign (basic 1) (private 1)) (public 1).
+
+Eval compute in check_dec (sign (basic 1) (private 1)) (public 2).
+
+Notation " 'good' " := (left _ _).
+
+Notation " 'bad' " := (right _ _).
+
+Eval compute in check_dec (sign (basic 1) (private 1)) (public 1).
+
+Eval compute in check_dec (sign (basic 1) (private 1)) (public 2).
+
+Theorem m2 : forall P Q R: Prop, P -> Q -> R -> Q.
+Proof.
+  intros. match goal with | [ B : _ |- _ ] => exact B end.
+Qed.                                                 
+
+(** [notHyp] determines if [P] is in the assumption set of a proof state.
+  The first match case simply checks to see if [P] matches any assumption and
+  fails if it does.  The second match case grabs everything else.  If [P]
+  is a conjunction, it checks to see if either of its conjuncts is an
+  assumption calling [notHyp] recursively. 
+
+*)
+
+Ltac notHyp P :=
+  match goal with
+  | [ _ : P |- _ ] => fail 1
+  | _ =>
+    match P with
+    | ?P1 /\ ?P2 => first [ notHyp P1 | notHyp P2 | fail 2 ]
+    | _ => idtac
+    end
+  end.
+                           
+Ltac extend pf :=
+  let t := type of pf in
+  notHyp t; generalize pf; intro.
